Compiler.thy
@@ -1,9 +1,9 @@
 theory Compiler
-  imports "01Source/AlgorithmicTypechecking" Printing "03Stack/StackConversion"
+  imports "01Source/AlgorithmicTypechecking" Printing "03Stack/StackConversion" 
 begin
 
 definition complete_compile :: "nexpr \<Rightarrow> byte_code list" where
-  "complete_compile = flatten_code \<circ> compile \<circ> convert"
+  "complete_compile = flatten_code \<circ> tco \<circ> compile \<circ> convert"
 
 theorem tc_terminationn: "typechecks e \<Longrightarrow> complete_compile e = cd \<Longrightarrow> 
   \<exists>v. valn v \<and> iter (\<leadsto>\<^sub>n) e v \<and> 
@@ -24,18 +24,23 @@ proof -
   with VN have VC: "print_closure c = print_nexpr v\<^sub>n" by simp
   from TC EC have "iter (\<leadsto>\<^sub>t) (compile_state (CSE [CReturn []] [] (convert e))) 
     (compile_state (CSC [] c))" by (metis iter_completet)
-  hence ET: "iter (\<leadsto>\<^sub>t) (TS [] [[]] (compile (convert e))) (TS [compile_closure c] [] [])" 
-    by simp
+  hence "iter (\<leadsto>\<^sub>t) (TS [] [[]] (compile (convert e))) (TS [compile_closure c] [] [])" 
+    by (simp add: compile_def)
+  hence "iter (\<leadsto>\<^sub>t) (tco_state (TS [] [[]] (compile (convert e)))) 
+    (tco_state (TS [compile_closure c] [] []))" by (metis iter_tco_eval )
+  hence ET: "iter (\<leadsto>\<^sub>t) (TS [] [[]] (tco (compile (convert e)))) 
+    (TS [tco_val (compile_closure c)] [] [])" by simp
   assume "complete_compile e = cd"
-  hence C: "flatten_code (compile (convert e)) = cd" by (simp add: complete_compile_def)
-  hence "unflatten_code cd (length cd) = compile (convert e)" by auto
-  hence UB: "unflatten_state (BS [] [[]] [length cd] cd) = TS [] [[]] (compile (convert e))" by simp
+  hence C: "flatten_code (tco (compile (convert e))) = cd" by (simp add: complete_compile_def)
+  hence "unflatten_code cd (length cd) = tco (compile (convert e))" by auto
+  hence UB: "unflatten_state (BS [] [[]] [length cd] cd) = TS [] [[]] (tco (compile (convert e)))" 
+    by simp
   from C have "orderly_state (BS [] [[]] [length cd] cd)" by auto
   with ET UB obtain v\<^sub>b where EB: 
     "iter (\<leadsto>\<^sub>b) (BS [] [[]] [length cd] cd) (BS [v\<^sub>b] [] [] cd) \<and> 
-      compile_closure c = unflatten_closure cd v\<^sub>b" 
+      tco_val (compile_closure c) = unflatten_closure cd v\<^sub>b" 
     by (metis evalb_end byte_code_state.sel(4))
-  hence "print_bclosure v\<^sub>b = print_tclosure (compile_closure c)" by simp
+  hence "print_bclosure v\<^sub>b = print_tclosure (tco_val (compile_closure c))" by simp
   with VC have VB: "print_bclosure v\<^sub>b = print_nexpr v\<^sub>n" by simp
   from EB obtain \<Sigma>\<^sub>h' where EH: "iter (\<leadsto>\<^sub>h) (HS hempty [] [[]] [length cd] cd) \<Sigma>\<^sub>h' \<and> 
     BS [v\<^sub>b] [] [] cd = unheap \<Sigma>\<^sub>h'" by fastforce
